pretty notation

Semantics/Imp/Aexp.lean
@@ -3,25 +3,25 @@ import Semantics.Imp.Lang
 namespace Aexp
 namespace Natural
 
-inductive step: Aexp → State → Val → Prop
+inductive step: Aexp → State → Int → Prop
   | val: step (val n) _ n
   | var: step (var x) s (s x)
   | add (ha: step a s n) (hb: step b s m):
-    step (add a b) s (n + m)
+    step (a + b) s (n + m)
   | sub (ha: step a s n) (hb: step b s m):
-    step (sub a b) s (n - m)
+    step (a - b) s (n - m)
   | mul (ha: step a s n) (hb: step b s m):
-    step (mul a b) s (n * m)
+    step (a * b) s (n * m)
 
 notation s " ⊢ " a " ⟹ " v => step a s v
 
 end Natural
 
 @[reducible]
-def reduce (a: Aexp) (s: State): Val :=
+def reduce (a: Aexp) (s: State): Int :=
   match a with
-  | val n => n
-  | var x => s x
+  | val a => a
+  | var a => s a
   | add a b => reduce a s + reduce b s
   | sub a b => reduce a s - reduce b s
   | mul a b => reduce a s * reduce b s
@@ -31,35 +31,40 @@ infix:100 "⇓" => reduce
 -- relational definition is equal to recursive
 theorem reduce.from_natural (h: s ⊢ a ⟹ n): a⇓s = n :=
   by induction h with
-  | add _ _ ih₁ ih₂ => exact ih₁ ▸ ih₂ ▸ rfl
-  | sub _ _ ih₁ ih₂ => exact ih₁ ▸ ih₂ ▸ rfl
-  | mul _ _ ih₁ ih₂ => exact ih₁ ▸ ih₂ ▸ rfl
+  | add _ _ iha ihb => exact iha ▸ ihb ▸ rfl
+  | sub _ _ iha ihb => exact iha ▸ ihb ▸ rfl
+  | mul _ _ iha ihb => exact iha ▸ ihb ▸ rfl
   | _ => rfl
 
 theorem Natural.from_reduce {a: Aexp} (h: a⇓s = n): s ⊢ a ⟹ n :=
   by induction a generalizing n with
-  | val _ => exact h ▸ step.val
-  | var _ => exact h ▸ step.var
-  | add _ _ l r => exact h ▸ step.add (l rfl) (r rfl)
-  | sub _ _ l r => exact h ▸ step.sub (l rfl) (r rfl)
-  | mul _ _ l r => exact h ▸ step.mul (l rfl) (r rfl)
+  | val a => exact h ▸ step.val
+  | var a => exact h ▸ step.var
+  | add a b iha ihb => exact h ▸ step.add (iha rfl) (ihb rfl)
+  | sub a b iha ihb => exact h ▸ step.sub (iha rfl) (ihb rfl)
+  | mul a b iha ihb => exact h ▸ step.mul (iha rfl) (ihb rfl)
 
-@[simp] theorem step_iff_reduce: (s ⊢ a ⟹ n) ↔ a⇓s = n := ⟨reduce.from_natural, Natural.from_reduce⟩
-@[simp] theorem step_iff_reduce': s ⊢ a ⟹ (a⇓s) := Natural.from_reduce rfl
+@[simp]
+theorem step_iff_reduce: (s ⊢ a ⟹ n) ↔ a⇓s = n :=
+  ⟨reduce.from_natural, Natural.from_reduce⟩
+@[simp]
+theorem step_iff_reduce': s ⊢ a ⟹ (a⇓s) :=
+  Natural.from_reduce rfl
 
 protected instance step.equiv: Setoid Aexp where
   r a b := ∀ s n, (s ⊢ a ⟹ n) = (s ⊢ b ⟹ n)
   iseqv := {
-    refl := fun _ _ _ => Eq.refl _
-    symm := fun h s n => Eq.symm (h s n)
-    trans := fun h₁ h₂ x n => (h₁ x n) ▸ (h₂ x n)
+    refl := fun _ _ _ => rfl
+    symm := fun h s n => (h s n).symm
+    trans := fun h1 h2 x n => (h1 x n) ▸ (h2 x n)
   }
 
 instance reduce.equiv: Setoid Aexp where
   r a b := ∀s, a⇓s = b⇓s
-  iseqv := ⟨fun _ _ => Eq.refl _, (Eq.symm $ · ·) , fun h₁ h₂ s => (h₁ s) ▸ (h₂ s)⟩
+  iseqv := ⟨fun _ _ => rfl, (Eq.symm $ · ·), fun h1 h2 s => (h1 s) ▸ (h2 s)⟩
 
-protected theorem step_eq_eq_reduce_eq: step.equiv.r a b ↔ reduce.equiv.r a b := by
+protected theorem step_eq_eq_reduce_eq:
+  step.equiv.r a b ↔ reduce.equiv.r a b := by
   constructor <;> intro h
   . simp [Setoid.r] at *
     intro s
