Semantics/Imp/Bexp.lean
@@ -7,32 +7,30 @@ namespace Natural
 inductive step: Bexp → State → Bool → Prop
   | tt: step tt _ true
   | ff: step ff _ false
-  | not
-    (h: step a s n):
-    step (not a) s (!n)
-  | and
-    (h₁: step a s n) (h₂: step b s m):
-    step (and a b) s (n && m)
-  | or
-    (h₁: step a s n) (h₂: step b s m):
-    step (or a b) s (n || m)
-  | eq: step (eq a b) s (a⇓s = b⇓s)
-  | le: step (le a b) s (a⇓s ≤ b⇓s)
+  | not (h: step a s n):
+    step (!a) s (!n)
+  | and (h₁: step a s n) (h₂: step b s m):
+    step (a && b) s (n && m)
+  | or (h₁: step a s n) (h₂: step b s m):
+    step (a || b) s (n || m)
+  | eq: step (a == b) s (a⇓s == b⇓s)
+  | le: step (a <= b) s (a⇓s <= b⇓s)
 
 notation s " ⊢ " a " ⟹ " v => step a s v
 
 end Natural
 
 -- Denotational semantics of Bexp
-@[reducible, simp] def reduce (b: Bexp) (s: State): Bool :=
+@[reducible, simp]
+def reduce (b: Bexp) (s: State): Bool :=
   match b with
   | tt      => true
   | ff      => false
   | not b   => !reduce b s
   | and a b => reduce a s && reduce b s
-  | or a b => reduce a s || reduce b s
-  | eq a b  => a.reduce s = b.reduce s
-  | le a b  => a.reduce s ≤ b.reduce s
+  | or a b  => reduce a s || reduce b s
+  | eq a b  => a.reduce s == b.reduce s
+  | le a b  => a.reduce s <= b.reduce s
 
 infix:100 "⇓" => reduce
 
@@ -41,37 +39,40 @@ theorem Natural.from_reduce {b: Bexp} (h: b⇓s = x): s ⊢ b ⟹ x :=
   by induction b generalizing x with
   | tt => exact h ▸ step.tt
   | ff => exact h ▸ step.ff
-  | not _ ih => exact h ▸ step.not (ih rfl)
-  | and _ _ l r => exact h ▸ step.and (l rfl) (r rfl)
-  | or _ _ l r => exact h ▸ step.or (l rfl) (r rfl)
+  | not a ih => exact h ▸ step.not (ih rfl)
+  | and a b iha ihb => exact h ▸ step.and (iha rfl) (ihb rfl)
+  | or a b iha ihb => exact h ▸ step.or (iha rfl) (ihb rfl)
   | eq => exact h ▸ step.eq
   | le => exact h ▸ step.le
 
 theorem reduce.from_natural {b: Bexp} (h: s ⊢ b ⟹ x): b⇓s = x :=
   by induction h with
   | not _ ih => exact ih ▸ rfl
-  | and _ _ ih₁ ih₂ => exact ih₁ ▸ ih₂ ▸ rfl
-  | or _ _ ih₁ ih₂ => exact ih₁ ▸ ih₂ ▸ rfl
+  | and _ _ iha ihb => exact iha ▸ ihb ▸ rfl
+  | or _ _ iha ihb => exact iha ▸ ihb ▸ rfl
   | _ => rfl
 
-@[simp] theorem step_eq_reduce {b: Bexp}: (s ⊢ b ⟹ x) ↔ b⇓s = x := ⟨reduce.from_natural, Natural.from_reduce⟩
+@[simp]
+theorem step_eq_reduce {b: Bexp}: (s ⊢ b ⟹ x) ↔ b⇓s = x :=
+  ⟨reduce.from_natural, Natural.from_reduce⟩
 
-theorem not_true_eq_false: (!b⇓s) = (not b)⇓s := by simp
+theorem not_true_eq_false: (!b⇓s) = (!b)⇓s := by simp
 
 protected instance step.equiv: Setoid Bexp where
   r a b := ∀ s n, Natural.step a s n = Natural.step b s n
   iseqv := {
-    refl := fun _ _ _ => Eq.refl _
-    symm := fun h s n => Eq.symm (h s n)
-    trans := fun h₁ h₂ x n => (h₁ x n) ▸ (h₂ x n)
+    refl := fun _ _ _ => rfl
+    symm := fun h s n => (h s n).symm
+    trans := fun h1 h2 x n => (h1 x n) ▸ (h2 x n)
   }
 
 @[reducible, simp]
 instance reduce.equiv: Setoid Bexp where
   r a b:= ∀s, a⇓s = b⇓s
-  iseqv := ⟨fun _ _ => Eq.refl _, (Eq.symm $ · ·) , fun h₁ h₂ s => (h₁ s) ▸ (h₂ s)⟩
+  iseqv := ⟨fun _ _ => rfl, (Eq.symm $ · ·), fun h1 h2 s => (h1 s) ▸ (h2 s)⟩
 
-protected theorem step_eq_eq_reduce_eq: step.equiv.r a b ↔ reduce.equiv.r a b := by
+protected theorem step_eq_eq_reduce_eq:
+  step.equiv.r a b ↔ reduce.equiv.r a b := by
   constructor <;> intro h
   . simp [Setoid.r] at *
     intro s
