Semantics/Imp/Lang.lean
@@ -1,9 +1,6 @@
 import Semantics.Maps
 
-@[reducible]
-def Val := Int
-
-def State := TotalMap Val
+def State := TotalMap Int
 def State.nil: State := TotalMap.default 0
 
 notation "σ₀" => State.nil
@@ -15,7 +12,7 @@ notation "σ₀" => State.nil
 example: σ₀⟪"x" ≔ 3⟫ = σ₀⟪"x" ≔ 4⟫⟪"x" ≔ 3⟫ := clobber.symm
 
 inductive Aexp where
-  | val : Val → Aexp
+  | val : Int → Aexp
   | var : String → Aexp
   -- arithmetic
   | add : Aexp → Aexp → Aexp
@@ -23,7 +20,7 @@ inductive Aexp where
   | mul : Aexp → Aexp → Aexp
 
 -- x + 3
-#check Aexp.add (Aexp.val 3) (Aexp.var "x")
+#check Aexp.add (Aexp.var "x") (Aexp.val 3)
 
 inductive Bexp where
   -- constants
@@ -47,29 +44,47 @@ inductive Com where
   | cond  : Bexp → Com → Com → Com
   | loop  : Bexp → Com → Com
 
+/-
+## Syntax
+-/
 -- Meta syntax
-notation:50 x:50 ";;" e:51 => Com.cat x e
+-- aexp
+notation:60 a:55 " * " b:56 => Aexp.mul a b
+notation:60 a:60 " + " b:61 => Aexp.add a b
+notation:60 a:60 " - " b:61 => Aexp.sub a b
+-- bexp
+notation:65 a:65 " && " b:66 => Bexp.and a b
+notation:65 a:65 " || " b:66 => Bexp.or a b
+notation:70 a:70 " == " b:71 => Bexp.eq a b
+notation:70 a:70 " <= " b:71 => Bexp.le a b
+notation:80 "!" a:81 => Bexp.not a
+-- com
+notation a:40 ";;" b:41 => Com.cat a b
+notation:50 a:50 " = " b:51 => Com.ass a b
+notation "if " c " then " a " else " b "end" => Com.cond c a b
+notation "while " c " loop " a "end" => Com.loop c a
 
--- Syntax of the language
 declare_syntax_cat imp
 
 -- general
 syntax "(" imp ")" : imp
--- imp
+-- aexp
 syntax num: imp
 syntax ident: imp
+syntax:55 imp:55 "*" imp:56 : imp
 syntax:60 imp:60 "+" imp:61 : imp
-syntax:60 imp:60 "-" imp:61: imp
+syntax:60 imp:60 "-" imp:61 : imp
 -- bexp
-syntax:80 "!" imp:81 : imp
-syntax:70 imp:70 "<=" imp:71 : imp
 syntax:65 imp:65 "&&" imp:66 : imp
--- stmt
-syntax:50 imp:50 "=" imp:51 : imp
+syntax:65 imp:65 "||" imp:66 : imp
+syntax:70 imp:70 "==" imp:71 : imp
+syntax:70 imp:70 "<=" imp:71 : imp
+syntax:80 "!" imp:81 : imp
+-- com
 syntax:40 imp:40 ";" imp:41 : imp
+syntax:50 imp:50 "=" imp:51 : imp
 syntax "if" imp "{" imp "}" "else" "{" imp "}" : imp
 syntax "while" imp "{" imp "}" : imp
-
 -- meta
 syntax "⦃" imp "⦄" : term
 
@@ -80,16 +95,19 @@ macro_rules
   | `(⦃false⦄) => `(Bexp.ff)
   -- general
   | `(⦃($x)⦄) => `(⦃$x⦄)
-  -- imp
+  -- aexp
   | `(⦃$x:ident⦄) => `(Aexp.var $(Lean.quote (toString x.getId)))
   | `(⦃$n:num⦄)   => `(Aexp.val $n)
   | `(⦃$x + $y⦄)  => `(Aexp.add ⦃$x⦄ ⦃$y⦄)
-  | `(⦃$x - $y⦄)  => `(Aexp.add ⦃$x⦄ ⦃$y⦄)
+  | `(⦃$x - $y⦄)  => `(Aexp.sub ⦃$x⦄ ⦃$y⦄)
+  | `(⦃$x * $y⦄)  => `(Aexp.mul ⦃$x⦄ ⦃$y⦄)
   -- bexp
   | `(⦃!$x⦄)      => `(Bexp.not ⦃$x⦄)
-  | `(⦃$x <= $y⦄)  => `(Bexp.le ⦃$x⦄ ⦃$y⦄)
   | `(⦃$x && $y⦄)  => `(Bexp.and ⦃$x⦄ ⦃$y⦄)
-  -- stmt
+  | `(⦃$x || $y⦄)  => `(Bexp.or ⦃$x⦄ ⦃$y⦄)
+  | `(⦃$x == $y⦄)  => `(Bexp.eq ⦃$x⦄ ⦃$y⦄)
+  | `(⦃$x <= $y⦄)  => `(Bexp.le ⦃$x⦄ ⦃$y⦄)
+  -- com
   | `(⦃$x:ident = $y⦄) => `(Com.ass $(Lean.quote (toString x.getId)) ⦃$y⦄)
   | `(⦃$x ; $y⦄)       => `(Com.cat ⦃$x⦄ ⦃$y⦄)
   | `(⦃if $b {$x} else {$y}⦄) => `(Com.cond ⦃$b⦄ ⦃$x⦄ ⦃$y⦄)
