Semantics/Imp/Natural.lean
@@ -8,27 +8,28 @@ inductive step: Com → State → State → Prop
     step skip s s
 
   | ass:
-    step (ass x a) s (s⟪x ≔ a⇓s⟫)
+    step (x = a) s (s⟪x ≔ a⇓s⟫)
 
   | cat t
     (hc: step c s t) (hd: step d t u):
-    step (cat c d) s u
+    step (c;;d) s u
 
-  | cond₁ {b: Bexp}
+  | cond_true {b: Bexp}
     (hb: b⇓s = true) (hc: step c s t):
-    step (cond b c d) s t
+    step if b then c else d end s t
 
-  | cond₂ {b: Bexp}
+  | cond_false {b: Bexp}
     (hb: b⇓s = false) (hd: step d s t):
-    step (cond b c d) s t
+    step if b then c else d end s t
 
-  | loop₁ {b: Bexp} u
-    (hb: b⇓s = true) (hc: step c s u) (hw: step (loop b c) u t):
-    step (loop b c) s t
+  | loop_true {b: Bexp} u
+    (hb: b⇓s = true) (hc: step c s u)
+    (hw: step while b loop c end u t):
+    step while b loop c end s t
 
-  | loop₂ {b: Bexp}
+  | loop_false {b: Bexp}
     (hb: b⇓s = false):
-    step (loop b c) s s
+    step while b loop c end s s
 
 notation:10 s " ⊢ " c " ⟹ " t => step c s t
 
@@ -38,59 +39,69 @@ private def z := "z"
 private example: σ₀ ⊢ ⦃x = 5⦄ ⟹ σ₀⟪x ≔ 5⟫ := step.ass
 private example:
   σ₀ ⊢ ⦃x = 2; if x <= 1 {y = 3} else {z = 4}⦄ ⟹ σ₀⟪x ≔ 2⟫⟪z ≔ 4⟫ :=
-    step.cat _ step.ass $ step.cond₂ rfl step.ass
+    step.cat _ step.ass $ step.cond_false rfl step.ass
 private example:
   σ₀ ⊢ ⦃x = 2; x = 3⦄ ⟹ σ₀⟪x ≔ 3⟫ := by
-  have h₁: σ₀⟪x ≔ 3⟫ = σ₀⟪x ≔ 2⟫⟪x ≔ 3⟫ := overwr.symm
-  rw [h₁]
+  have h1: σ₀⟪x ≔ 3⟫ = σ₀⟪x ≔ 2⟫⟪x ≔ 3⟫ := clobber.symm
+  rw [h1]
   apply step.cat _ step.ass step.ass
 
 /-
 ## Rewriting rules
 -/
 
-theorem skip_iff: (s ⊢ skip ⟹ t) ↔ s = t := by
-  apply Iff.intro <;> intro h
+theorem skip_iff: (s ⊢ skip ⟹ t) = (s = t) := by
+  apply propext
+  constructor <;> intro h
   . cases h; rfl
   . exact h ▸ step.skip
 
-theorem cat_iff: (s ⊢ c;;d ⟹ t) ↔ ∃ w, (s ⊢ c ⟹ w) ∧ (w ⊢ d ⟹ t) := by
-  apply Iff.intro <;> intro h
-  . cases h with | cat t h₁ h₂ =>
-      exact ⟨t, ⟨h₁, h₂⟩⟩
-  . cases h with | intro w h =>
-      exact step.cat w h.1 h.2
-
-theorem cond_iff: (s ⊢ cond b c d ⟹ t) ↔ bif b⇓s then (s ⊢ c ⟹ t) else (s ⊢ d ⟹ t) := by
+theorem cat_iff:
+  (s ⊢ c;;d ⟹ t) = ∃ w, (s ⊢ c ⟹ w) ∧ (w ⊢ d ⟹ t) := by
+  apply propext
   constructor <;> intro h
   . cases h with
-    | cond₁ hb hc => exact hb ▸ hc
-    | cond₂ hb hc => exact hb ▸ hc
-  . cases hb: b⇓s with
-    | true => exact step.cond₁ hb $ (cond_true (s ⊢ c ⟹ t) _) ▸ hb ▸ h
-    | false => exact step.cond₂ hb $ (cond_false _ (s ⊢ d ⟹ t)) ▸ hb ▸ h
+    | cat t h1 h2 =>
+      exact ⟨t, ⟨h1, h2⟩⟩
+  . cases h with
+    | intro w h =>
+      exact step.cat w h.1 h.2
 
-theorem cond_iff': (s ⊢ cond b c d ⟹ t) ↔ (s ⊢ bif b⇓s then c else d ⟹ t) := by
+theorem cond_iff:
+  (s ⊢ if b then c else d end ⟹ t)
+    = bif b⇓s then (s ⊢ c ⟹ t) else (s ⊢ d ⟹ t) := by
+  apply propext
+  constructor <;> intro h
+  . cases h with
+    | cond_true hb hc => exact hb ▸ hc
+    | cond_false hb hc => exact hb ▸ hc
+  . cases hb: b⇓s with
+    | true => exact step.cond_true hb $ (cond_true (s ⊢ c ⟹ t) _) ▸ hb ▸ h
+    | false => exact step.cond_false hb $ (cond_false _ (s ⊢ d ⟹ t)) ▸ hb ▸ h
+
+theorem cond_iff':
+  (s ⊢ if b then c else d end ⟹ t)
+    = (s ⊢ bif b⇓s then c else d ⟹ t) := by
   rw [cond_iff]
   cases b⇓s with
   | false => rw [cond_false, cond_false]
   | true => rw [cond_true, cond_true]
 
-theorem loop_iff: (s ⊢ loop b c ⟹ t) ↔
-  bif b⇓s then ∃ w, (s ⊢ c ⟹ w) ∧ (w ⊢ loop b c ⟹ t) else s = t := by
-  apply Iff.intro <;> intro h
+theorem loop_iff: (s ⊢ while b loop c end ⟹ t) =
+  bif b⇓s then ∃w, (s ⊢ c ⟹ w) ∧ (w ⊢ while b loop c end ⟹ t) else s = t := by
+  apply propext
+  constructor <;> intro h
   . cases h with
-    | loop₁ t hb hc hw =>
-      exact hb ▸ ⟨t, ⟨hc, hw⟩⟩
-    | loop₂ hb =>
-      exact hb ▸ rfl
+    | loop_true t hb hc hw => exact hb ▸ ⟨t, ⟨hc, hw⟩⟩
+    | loop_false hb => exact hb ▸ rfl
   . cases hb: b⇓s with
     | true =>
       rw [hb] at h
-      cases h with | intro w h =>
-        exact step.loop₁ w hb h.1 h.2
+      cases h with
+      | intro w h =>
+        exact step.loop_true w hb h.1 h.2
     | false =>
-      exact (hb ▸ h) ▸ step.loop₂ hb
+      exact (hb ▸ h) ▸ step.loop_false hb
 
 /-
 ## Behavioral equivalence
@@ -99,15 +110,17 @@ theorem loop_iff: (s ⊢ loop b c ⟹ t) ↔
 instance equiv: Setoid Com where
   r c d := ∀ s t, (s ⊢ c ⟹ t) ↔ (s ⊢ d ⟹ t)
   iseqv := {
-    refl := fun _ _ _ => Iff.refl _
+    refl := fun _ _ _ => Iff.rfl
     symm := (Iff.symm $ · · ·)
-    trans := fun h₁ h₂ x n => Iff.trans (h₁ x n) (h₂ x n)
+    trans := fun h1 h2 x n => Iff.trans (h1 x n) (h2 x n)
   }
 
 theorem skipl: (skip;;c) ≈ c := by
   intro _ _
   constructor
-  . intro h; cases h with | cat _ hc hd =>
+  . intro h
+    cases h with
+    | cat _ hc hd =>
       exact skip_iff.mp hc ▸ hd
   . exact (step.cat _ step.skip ·)
 
@@ -118,24 +131,24 @@ theorem skipr: (c;;skip) ≈ c := by
       exact skip_iff.mp hd ▸ hc
   . exact (step.cat _ · step.skip)
 
-theorem cond_true (h: b ≈ Bexp.tt): cond b c d ≈ c := by
+theorem cond_true (h: b ≈ Bexp.tt): if b then c else d end ≈ c := by
   intro _ _
   rw [cond_iff, h]
-  exact Iff.rfl
+  rfl
 
-theorem cond_false (h: b ≈ Bexp.ff): cond b c d ≈ d := by
+theorem cond_false (h: b ≈ Bexp.ff): if b then c else d end ≈ d := by
   intro _ _
   rw [cond_iff, h]
-  exact Iff.rfl
+  rfl
 
 theorem loop_unfold:
-  loop b c ≈ cond b (c;;loop b c) skip := by
+  while b loop c end ≈ if b then (c;;while b loop c end) else skip end := by
   intro s t
-  apply Iff.intro <;> intro h
+  constructor <;> intro h
   . rw [cond_iff]
     cases h with
-    | loop₁ w hb hc hw => exact hb ▸ step.cat w hc hw
-    | loop₂ hb => exact hb ▸ step.skip
+    | loop_true w hb hc hw => exact hb ▸ step.cat w hc hw
+    | loop_false hb => exact hb ▸ step.skip
   . rw [loop_iff]
     rw [cond_iff] at h
     cases hb: b⇓s <;> rw [hb] at h
@@ -147,35 +160,53 @@ theorem loop_unfold:
 -/
 
 theorem loop_tt (h: b ≈ Bexp.tt):
-  ¬(s ⊢ loop b c ⟹ t) := by
-  intro h₁
-  generalize h₂: loop b c = ww at h₁
-  induction h₁ with
-  | loop₁ _ _ _ _ _ ih₂ => cases h₂; apply ih₂; rfl
-  | loop₂ hb => cases h₂; rw [h] at hb; contradiction
-  | _ => cases h₂
+  ¬(s ⊢ while b loop c end ⟹ t) := by
+  intro h1
+  generalize h2: while b loop c end = ww at h1
+  induction h1 with
+  | loop_true _ _ _ _ _ ih2 => cases h2; apply ih2; rfl
+  | loop_false hb => cases h2; rw [h] at hb; contradiction
+  | _ => cases h2
 
 /-
 ## Determinism
 -/
 
-theorem deterministic {c: Com} (h₁: w ⊢ c ⟹ s) (h₂: w ⊢ c ⟹ t): s = t :=
-  by induction h₁ generalizing t with
-  | cat _ _ _ ih₁ ih₂ => cases h₂ with
-    | cat _ hc hd => exact ih₂ (ih₁ hc ▸ hd)
-  | cond₁ hb _ ih => cases h₂ with
-    | cond₁ _ hd => exact ih hd
-    | cond₂ hb₁ hd => rw [hb] at hb₁; contradiction
-  | cond₂ hb _ ih => cases h₂ with
-    | cond₁ hb₁ hd => rw [hb] at hb₁; contradiction
-    | cond₂ _ hd   => exact ih hd
-  | loop₁ _ hb _ _ ih₁ ih₂ => cases h₂ with
-    | loop₁ _ _ hc hw => exact ih₂ (ih₁ hc ▸ hw)
-    | loop₂ hb₁ => rw [hb] at hb₁; contradiction
-  | loop₂ hb => cases h₂ with
-    | loop₁ _ hb₁ => rw [hb] at hb₁; contradiction
-    | loop₂ => rfl
-  | _ => cases h₂; rfl
+theorem deterministic {c: Com}
+  (h1: w ⊢ c ⟹ s) (h2: w ⊢ c ⟹ t): s = t :=
+  by induction h1 generalizing t with
+  | cat _ _ _ ihc ihd =>
+    cases h2 with
+    | cat _ hc hd =>
+      exact ihd (ihc hc ▸ hd)
+  | cond_true hb _ ih =>
+    cases h2 with
+    | cond_true _ hd =>
+      exact ih hd
+    | cond_false hb1 hd =>
+      rw [hb] at hb1
+      contradiction
+  | cond_false hb _ ih =>
+    cases h2 with
+    | cond_true hb1 hd =>
+      rw [hb] at hb1
+      contradiction
+    | cond_false _ hd =>
+      exact ih hd
+  | loop_true _ hb _ _ ihc ihw =>
+    cases h2 with
+    | loop_true _ _ hc hw =>
+      exact ihw (ihc hc ▸ hw)
+    | loop_false hb1 =>
+      rw [hb] at hb1
+      contradiction
+  | loop_false hb =>
+    cases h2 with
+    | loop_true _ hb1 =>
+      rw [hb] at hb1
+      contradiction
+    | loop_false => rfl
+  | _ => cases h2; rfl
 
 end Natural
 end Com
